James C - constraints mostly ready

isabelle/Chapter12_2_PatternMatching.thy
@@ -32,4 +32,73 @@ where "no_match p1 e1 ==> no_match (PairPat p1 p2) (Pair e1 e2)"
     | "no_match (InRPat p) (InL t t' e)"
     | "no_match p e ==> no_match (InRPat p) (InR t t' e)"
 
+datatype constraint = 
+  Truth
+| Falsity
+| And constraint constraint
+| Or constraint constraint
+| InLCon constraint
+| InRCon constraint
+| TrivCon
+| PairCon constraint constraint
+
+primrec patn_constraint :: "patn => constraint"
+where "patn_constraint VarPat = Truth"
+    | "patn_constraint WildPat = Truth"
+    | "patn_constraint TrivPat = TrivCon"
+    | "patn_constraint (PairPat p1 p2) = PairCon (patn_constraint p1) (patn_constraint p2)"
+    | "patn_constraint (InLPat p) = InLCon (patn_constraint p)"
+    | "patn_constraint (InRPat p) = InRCon (patn_constraint p)"
+
+fun rule_constraint :: "rule => constraint"
+where "rule_constraint (Rule p e) = patn_constraint p"
+
+primrec rules_constraint :: "rule list => constraint"
+where "rules_constraint [] = Falsity"
+    | "rules_constraint (r # rs) = Or (rule_constraint r) (rules_constraint rs)"
+
+primrec negate :: "constraint => constraint"
+where "negate Truth = Falsity"
+    | "negate Falsity = Truth"
+    | "negate (And c1 c2) = Or (negate c1) (negate c2)"
+    | "negate (Or c1 c2) = And (negate c1) (negate c2)"
+    | "negate (InLCon c) = Or (InLCon (negate c)) (InRCon Truth)"
+    | "negate (InRCon c) = Or (InRCon (negate c)) (InLCon Truth)"
+    | "negate TrivCon = Falsity"
+    | "negate (PairCon c1 c2) = Or (PairCon c1 (negate c2)) 
+                               (Or (PairCon (negate c1) c2) 
+                                   (PairCon (negate c1) (negate c2)))"
+
+fun is_incon :: "constraint list => bool"
+where "is_incon [] = False"
+    | "is_incon (Truth # cs) = is_incon cs"
+    | "is_incon (Falsity # cs) = True"
+    | "is_incon (And c1 c2 # cs) = undefined"
+    | "is_incon (Or c1 c2 # cs) = undefined"
+    | "is_incon (InLCon c # cs) = undefined"
+    | "is_incon (InRCon c # cs) = undefined"
+    | "is_incon (TrivCon # cs) = undefined"
+    | "is_incon (PairCon c1 c2 # cs) = undefined"
+
+definition satisfies_all :: "constraint => bool"
+where "satisfies_all c = is_incon [negate c]"
+
+lemma [simp]: "rule_constraint (insert_rule n r) = rule_constraint r"
+by (induction r, simp_all)
+
+lemma [simp]: "rules_constraint (insert_rules n rs) = rules_constraint rs"
+by (induction rs, simp_all)
+
+lemma [simp]: "rule_constraint (subst_rule n e r) = rule_constraint r"
+by (induction r, simp_all)
+
+lemma [simp]: "rules_constraint (subst_rules n e rs) = rules_constraint rs"
+by (induction rs, simp_all)
+
+lemma [simp]: "rule_constraint (remove_rule n r) = rule_constraint r"
+by (induction r, simp_all)
+
+lemma [simp]: "rules_constraint (remove_rules n rs) = rules_constraint rs"
+by (induction rs, simp_all)
+
 end
